and_list_true_implies_element_in_list_true proven. Alea code moved to separate file

proofs.v
@@ -1,7 +1,4 @@
-(* Add Rec LoadPath "/nix/store/ir85s7vq85gg888j3gkqvba411nxrjxf-coq8.15-alea/lib/coq/8.15+alpha/user-contrib/ALEA/" as ALEA. *)
 From Coq Require Export Arith.
-(* From ALEA Require Import Ccpo. *)
-(* From ALEA Require Import Choice. *)
 Set Implicit Arguments.
 Unset Strict Implicit.
 Require Coq.extraction.Extraction.
@@ -9,99 +6,184 @@ Extraction Language OCaml.
 Set Printing Projections.
 Require Import Bool.
 Require Import List.
+
 Inductive Correctness : Type :=
 | yes : Correctness
 | no : Correctness
 | trusted : Correctness
 | idk : Correctness.
+
 Inductive Node : Type := mkNode
                            { correctness : Correctness
                            ; children : list Node
                            }.
-(* Inductive DebuggingTree : Type := *)
-(*     right_neutral : forall x, x * 1 = x  *)
+
 Definition node1 := mkNode idk nil.
 Definition node2 := mkNode idk nil.
 Definition node3 := mkNode trusted (node1::node2::nil).
 Eval compute in correctness node3.
-(* Lemma list_sum_ge_0 : forall l : list nat, 0 <= list_sum l. *)
-(* Proof. intros l. induction l. simpl. intuition. simpl. assert (a >= 0). induction a. intuition. apply le_0_n.  subst. induction a. intuition.  *)
-(* Qed. *)
+Lemma list_sum_ge_0 : forall l : list nat, 0 <= list_sum l.
+Proof.
+  intros l.
+  induction l.
+  simpl.
+  intuition.
+  simpl.
+  assert (a >= 0).
+  induction a.
+  intuition.
+  apply le_0_n.
+  subst.
+  induction a.
+  intuition.
+  intuition.
+Qed.
+SearchPattern (Prop).
 Fixpoint and_list (l : list Prop) : Prop :=
   match l with
     nil => True
-  | n::tl => and n (and_list tl)
+  | hd::tl => and hd (and_list tl)
   end.
+
+Lemma and_list_true_implies_element_in_list_true: forall (A : Type) (l : list A) (element : A) (x : A -> Prop), and_list (map (fun item => x item) l) /\ In element l -> x element.
+Proof.
+  intros.
+  intuition.
+  induction l.
+  + inversion H1.
+  + destruct H1.
+    - subst.
+      inversion H0.
+      exact H.
+    - inversion H0. intuition.
+Qed.
+
 Eval compute in and_list (True::True::True::nil).
 Check 1::nil.
+
 Fixpoint weight (node : Node) : nat :=
-  match node.(children) with
-    nil => 1
-  | children => S (list_sum (map (fun child => weight child) (children)))
-  end.
-Lemma commutativity : forall a b:Prop, a/\b -> b/\a.
-Proof.
-  intros a b H. split. destruct H as [H1 H2]. exact H2. destruct H as [H1 H2]. exact H1.
-Qed.
+  S (list_sum (map (fun child => weight child) (children node))).
 
 Lemma weight_childfree_node_eq_1: forall n:Node, n.(children) = nil -> weight n = (S 0).
 Proof.
-  - intros n H. induction n. simpl. assert (children0 = nil). apply H. rewrite H0. reflexivity.
+  intros n H.
+  induction n.
+  simpl.
+  assert (children0 = nil).
+  exact H.
+  rewrite H0.
+  reflexivity.
 Qed.
 
 Lemma weight_gt_0: forall n:Node, 0 < weight n.
-Proof. intros n. induction n. induction children0. simpl. intuition. simpl. intuition.
+Proof.
+  intros n.
+  induction n.
+  induction children0.
+  + simpl.
+    intuition.
+  + simpl.
+    intuition.
 Qed.
+
 Search list.
 Require Import Lia.
 Search nat.
 
 Lemma node_weight_gt_sum_children_weight: forall n:Node, weight n > list_sum (map (fun child => weight child) (children n)).
-Proof. intros n. induction n. simpl. induction children0.
-       + simpl. destruct (zerop 1). discriminate. assumption.
-       + simpl. intuition.
+Proof.
+  intros n.
+  induction n.
+  simpl.
+  induction children0.
+  + simpl.
+    destruct (zerop 1).
+    discriminate.
+    exact l.
+  + simpl.
+    intuition.
 Qed.
 
 SearchPattern (_ <= _).
 Lemma nat_in_list_le_list_sum: forall (l:list nat) (element: nat), In element l -> element <= list_sum l.
-Proof. intros l element H. induction l.
-       - simpl. inversion H.
-       - simpl. destruct H.
-         + subst. apply Nat.le_add_r.
-         + transitivity (list_sum l);auto.
-           rewrite Nat.add_comm. apply Nat.le_add_r.
+Proof.
+  intros l element H.
+  induction l.
+  + simpl.
+    inversion H.
+  + simpl.
+    destruct H.
+    - subst.
+      apply Nat.le_add_r.
+    - transitivity (list_sum l);auto.
+      rewrite Nat.add_comm.
+      apply Nat.le_add_r.
 Qed.
 
 Lemma child_weight_le_sum_children_weight: forall (l:list Node) (child: Node), In child l -> list_sum (map (fun child => weight child) l) >= weight child.
-Proof. intros l child H. apply nat_in_list_le_list_sum. induction l.
-       - simpl. inversion H.
-       - simpl. destruct H.
-         + subst. intuition.
-         + subst. intuition.
+Proof.
+  intros l child H.
+  apply nat_in_list_le_list_sum.
+  induction l.
+  - simpl.
+    inversion H.
+  - simpl.
+    destruct H.
+    + subst.
+      intuition.
+    + subst.
+      intuition.
 Qed.
+
 SearchPattern (_ < _ + _).
 Lemma parent_weight_gt_child_weight: forall parent child:Node, In child (children parent) -> weight child < weight parent.
-Proof. intros parent child H. induction parent. simpl. induction children0.
-       + inversion H.
-       + inversion H.
-         - rewrite H0. intuition.
-         -  intuition. assert (weight child <= list_sum (map (fun child0 : Node => weight child0) children0)). apply child_weight_le_sum_children_weight. assumption. intuition. assert (weight a > 0). apply weight_gt_0. assert (weight child < (weight a + list_sum (map (fun child0 : Node => weight child0) children0))). inversion H2. rewrite Nat.add_comm. apply Nat.lt_add_pos_r. assumption. assert (weight child < S m). intuition. rewrite Nat.add_comm. intuition. intuition.
+Proof.
+  intros parent child H.
+  induction parent.
+  simpl.
+  induction children0.
+  + inversion H.
+  + inversion H.
+  - rewrite H0.
+    intuition.
+  - intuition.
+    assert (weight child <= list_sum (map (fun child0 : Node => weight child0) children0)).
+    apply child_weight_le_sum_children_weight.
+    exact H0.
+    assert (weight a > 0).
+    apply weight_gt_0.
+    assert (weight child < (weight a + list_sum (map (fun child0 : Node => weight child0) children0))).
+    inversion H2.
+    rewrite Nat.add_comm.
+    apply Nat.lt_add_pos_r.
+    exact H3.
+    assert (weight child < S m).
+    intuition.
+    rewrite Nat.add_comm.
+    intuition.
+    intuition.
 Qed.
 
 Eval compute in idk = idk.
 Scheme Equality for Correctness.
 Fixpoint are_all_idk (node : Node) : Prop :=
-  match node.(children) with
-    nil => node.(correctness) = idk
-  | children => and (node.(correctness) = idk) (and_list (map (fun child => are_all_idk child) (children)))
-  end.
+  and (node.(correctness) = idk) (and_list (map (fun child => are_all_idk child) (children node))).
+Eval compute in are_all_idk node3.
 
 Lemma are_all_idk_implies_children_all_idk: forall n : Node, are_all_idk n -> and_list (map (fun child => are_all_idk child) (children n)).
-Proof. intros n H. induction n. induction children0.
-       + inversion H. simpl. constructor.
-       + inversion H. simpl. split.
-       - inversion H. apply H3.
-       - apply H1.
+Proof.
+  intros n H.
+  induction n.
+  induction children0.
+  + inversion H.
+    simpl.
+    constructor.
+  + inversion H.
+    simpl.
+    split.
+  - inversion H.
+    apply H3.
+  - apply H1.
 Qed.
 
 Eval compute in are_all_idk node1.
@@ -111,7 +193,15 @@ Eval compute in are_all_idk node4.
 Definition is_debugging_tree (node : Node) : Prop :=
   and (node.(correctness) = no) (and_list (map (fun child => are_all_idk child) (children node))).
 
-(* Extraction pred. *)
+Lemma is_debugging_tree_true: forall node: Node, is_debugging_tree node -> and (node.(correctness) = no) (and_list (map (fun child => are_all_idk child) (children node))).
+Proof.
+  intros n H.
+  inversion H.
+  split.
+  + exact H0.
+  + exact H1.
+Qed.
+  (* Extraction pred. *)
 (* Extraction is_debugging_tree. *)
 
 Eval compute in is_debugging_tree node1.
@@ -181,13 +271,27 @@ Definition get_debugging_tree_from_tree (n : Node) : Node :=
   mkNode no (children n).
 Require Import Program.Wf.
 Lemma debugging_tree_of_tree_has_same_weight: forall n:Node, weight n = weight (get_debugging_tree_from_tree n).
-Proof. intros n. induction n. simpl. reflexivity.
+Proof.
+  intros n.
+  induction n.
+  simpl.
+  reflexivity.
 Qed.
+
 Lemma children_of_debugging_tree_remain_unchanged: forall n:Node, children n = children (get_debugging_tree_from_tree n).
-Proof. intros n. induction n. simpl. reflexivity.
+Proof.
+  intros n.
+  induction n.
+  simpl.
+  reflexivity.
 Qed.
+
 Lemma debugging_tree_root_node_is_incorrect: forall n:Node, correctness (get_debugging_tree_from_tree n) = no.
-Proof. intros n. induction n. simpl. reflexivity.
+Proof.
+  intros n.
+  induction n.
+  simpl.
+  reflexivity.
 Qed.
 
 Lemma debugging_tree_of_tree_with_all_children_idk_is_debugging_tree: forall n:Node, and_list (map (fun child => are_all_idk child) (children n)) -> is_debugging_tree (get_debugging_tree_from_tree n).
@@ -199,11 +303,12 @@ Proof.
   assert (correctness (get_debugging_tree_from_tree n) = no).
   apply debugging_tree_root_node_is_incorrect.
   assert (and_list (map (fun child : Node => are_all_idk child) (get_debugging_tree_from_tree n).(children))).
-       + rewrite <- H0. apply H.
+       + rewrite <- H0. exact H.
        + unfold is_debugging_tree. split.
-         - apply H1.
-         - apply H2.
+         - exact H1.
+         - exact H2.
 Qed.
+Require Import Lia.
 
 Lemma debugging_tree_of_idk_tree_is_debugging_tree: forall n:Node, are_all_idk n -> is_debugging_tree (get_debugging_tree_from_tree n).
 Proof.
@@ -213,11 +318,13 @@ Proof.
   + apply debugging_tree_root_node_is_incorrect.
   + assert (and_list (map (fun child : Node => are_all_idk child) n.(children))).
     apply are_all_idk_implies_children_all_idk.
-  - apply H.
-  - assert (children n = children (get_debugging_tree_from_tree n)). apply children_of_debugging_tree_remain_unchanged. rewrite <- H1. apply H0.
+  - exact H.
+  - assert (children n = children (get_debugging_tree_from_tree n)).
+    apply children_of_debugging_tree_remain_unchanged.
+    rewrite <- H1.
+    exact H0.
 Qed.
 
-Show Obligation Tactic.
 Obligation Tactic := intros.
 
 Program Fixpoint generic_debugging_algorithm (n : Node) {measure (weight n)}: Node :=
@@ -226,266 +333,92 @@ Program Fixpoint generic_debugging_algorithm (n : Node) {measure (weight n)}: No
   | head::tail => generic_debugging_algorithm (get_debugging_tree_from_tree head)
   end.
 Next Obligation.
-  assert (In head (children n)). induction (children n). inversion Heq_anonymous.  simpl. left. injection Heq_anonymous. intuition. assert (weight head = weight (get_debugging_tree_from_tree head)). apply debugging_tree_of_tree_has_same_weight. rewrite <- H0. apply parent_weight_gt_child_weight. assumption.
+  assert (In head (children n)).
+  + induction (children n).
+    - inversion Heq_anonymous.
+    - simpl.
+      left.
+      injection Heq_anonymous.
+      intuition.
+  + assert (weight head = weight (get_debugging_tree_from_tree head)).
+    - apply debugging_tree_of_tree_has_same_weight.
+    - rewrite <- H0.
+      apply parent_weight_gt_child_weight.
+      exact H.
 Qed.
 Next Obligation.
   intuition.
 Qed.
-Check generic_debugging_algorithm.
-Show Obligation Tactic.
+
+Obligation Tactic := intros.
 Obligation Tactic := Tactics.program_simpl.
-Show Obligation Tactic.
+Program Fixpoint generic_debugging_algorithm_dp (n : {n: Node | is_debugging_tree n}) {measure (weight n)}: Node :=
+  match children n with
+    nil => n
+  | head::tail => generic_debugging_algorithm_dp (get_debugging_tree_from_tree head)
+  end.
+Obligations of generic_debugging_algorithm_dp.
+Next Obligation.
+  inversion H.
+  assert (are_all_idk head).
+  + assert (In head (children n)).
+  - induction (children n).
+    inversion Heq_anonymous.
+    simpl.
+    left.
+    injection Heq_anonymous.
+    intuition.
+  - apply H1.
+      apply Heq_anonymous.
+  intuition.
+  assert (correctness head = idk).
+  +
+  intuition.
+  assert (is_debugging_tree (n)).
+  apply H.
+  + split.
+  - apply is_debugging_tree_true.
+    intuition.
+  apply debu
+  apply debugging_tree_of_idk_tree_is_debugging_tree.
+  assert (is_debugging_tree (n)).
+  Check n.
+  assert (and_list (map (fun child : Node => are_all_idk child) (proj1_sig n).(children))).
+  apply generic_debugging_algorithm_dp.
+  inversion n.
+  assert  (are_all_idk head).
+  assert (are_all_idk head).
+  assert (In head (children n)).
+  + induction (children n).
+    - inversion Heq_anonymous.
+    - simpl.
+      left.
+      injection Heq_anonymous.
+      intuition.
+  + assert (weight head = weight (get_debugging_tree_from_tree head)).
+    - apply debugging_tree_of_tree_has_same_weight.
+    - rewrite <- H0.
+      apply parent_weight_gt_child_weight.
+      exact H.
+Qed.
+Next Obligation.
+  intuition.
+Qed.
+
+
+
+Obligation Tactic := Tactics.program_simpl.
+
+Lemma generic_debugging_algorithm_returns_incorrect_childfree_node_when_given_debugging_tree: forall n:Node, is_debugging_tree n -> correctness (generic_debugging_algorithm n) = no.
+Proof.
+  intros n H.
+  induction n.
+  induction children0.
+  - cbv. intuition. simpl.
 
 Lemma generic_debugging_algorithm_returns_childfree_node: forall n:Node, children (generic_debugging_algorithm n) = nil.
-Proof. intros n. induction n. induction children0.
-       + unfold generic_debugging_algorithm. simpl. intuition. auto. eauto.
-
-
-Lemma generic_debugging_algorithm_returns_incorrect_childfree_node_when_given_debugging_tree: forall n:Node, eq_true (is_debugging_tree n) -> correctness (generic_debugging_algorithm n) = no.
-Proof. intros n H. intuition.
-       + induction n. induction children0.
-         - intuition. simpl.
-
-
-(* From ALEA Require Import Cover. *)
-(* (* From ALEA Require Import Misc. *) *)
-(* (* From ALEA Require Import Monads. *) *)
-(* (* From ALEA Require Import Probas. *) *)
-(* (* From ALEA Require Import Prog. *) *)
-(* (* From ALEA Require Import Sets. *) *)
-(* (* From ALEA Require Import Uprop. *) *)
-(* From ALEA Require Import Utheory. *)
-(* Module MyM (Univ : Universe). *)
-(*   Module Import Cover := CoverFun Univ. *)
-(*   Include Univ. *)
-(*   Export RP. *)
-(*   Export PP. *)
-(*   Set Implicit Arguments. *)
-(*   Unset Strict Implicit. *)
-(*   Require Coq.extraction.Extraction. *)
-(*   Extraction Language OCaml. *)
-(*   Set Printing Projections. *)
-(*   Require Import Bool. *)
-(*   Require Import List. *)
-(*   Inductive Correctness : Type := *)
-(*   | yes : Correctness *)
-(*   | no : Correctness *)
-(*   | trusted : Correctness *)
-(*   | idk : Correctness. *)
-(*   Inductive Node : Type := mkNode *)
-(*                              { correctness : Correctness *)
-(*                              ; children : list Node *)
-(*                              }. *)
-(*   (* Inductive DebuggingTree : Type := *) *)
-(*   (*     right_neutral : forall x, x * 1 = x  *) *)
-(*   Definition node1 := mkNode idk nil. *)
-(*   Definition node2 := mkNode idk nil. *)
-(*   Definition node3 := mkNode trusted (node1::node2::nil). *)
-(*   Eval compute in correctness node3. *)
-(*   (* Lemma list_sum_ge_0 : forall l : list nat, 0 <= list_sum l. *) *)
-(*   (* Proof. intros l. induction l. simpl. intuition. simpl. assert (a >= 0). induction a. intuition. apply le_0_n.  subst. induction a. intuition.  *) *)
-(*   (* Qed. *) *)
-(*   Fixpoint and_list (l : list bool) : bool := *)
-(*     match l with *)
-(*       nil => true *)
-(*     | n::tl => andb n (and_list tl) *)
-(*     end. *)
-(*   Eval compute in and_list (true::true::true::nil). *)
-(*   Check 1::nil. *)
-(*   Fixpoint weight (node : Node) : nat := *)
-(*     match node.(children) with *)
-(*       nil => 1 *)
-(*     | children => 1 + list_sum (map (fun child => weight child) (children)) *)
-(*     end. *)
-(*   Lemma commutativity : forall a b:Prop, a/\b -> b/\a. *)
-(*   Proof. *)
-(*     intros a b H. split. destruct H as [H1 H2]. exact H2. intuition. *)
-(*   Qed. *)
-
-(*   Lemma weight_childfree_node_eq_1: forall n:Node, n.(children) = nil -> weight n = (S 0). *)
-(*   Proof. *)
-(*     - intros n H. induction n. simpl. assert (children0 = nil). apply H. subst. reflexivity. *)
-(*   Qed. *)
-
-(*   (* Lemma weight_g_0: forall n:Node, 0 < weight n. *) *)
-(*   (* Proof. intros n. induction n. induction children0. simpl. intuition. simpl. intuition. *) *)
-(*   (* Qed. *) *)
-(*   Eval compute in idk = idk. *)
-(*   Scheme Equality for Correctness. *)
-(*   Fixpoint are_all_idk (node : Node) : bool := *)
-(*     match node.(children) with *)
-(*       nil => Correctness_beq node.(correctness) idk *)
-(*     | children => andb (Correctness_beq node.(correctness) idk) (and_list (map (fun child => are_all_idk child) (children))) *)
-(*     end. *)
-(*   Eval compute in are_all_idk node1. *)
-(*   Definition node4 := mkNode idk (node1::node2::nil). *)
-(*   Eval compute in are_all_idk node4. *)
-(*   Definition is_debugging_tree (node : Node) : bool := *)
-(*     match node.(children) with *)
-(*       nil => Correctness_beq node.(correctness) no *)
-(*     | children => andb (Correctness_beq node.(correctness) no) (and_list (map (fun child => are_all_idk child) (children))) *)
-(*     end. *)
-(*   (* Extraction pred. *) *)
-(*   (* Extraction is_debugging_tree. *) *)
-
-(*   Eval compute in is_debugging_tree node1. *)
-(*   Definition node5 := mkNode no (node1::nil). *)
-(*   Eval compute in is_debugging_tree node5. *)
-(*   (* Eval compute in list_sum (map (fun x => x + 3) (1::2::5::nil)). *) *)
-(*   Eval compute in weight node3. *)
-(*   Eval compute in is_debugging_tree node5. *)
-(*   Check andb (is_debugging_tree node1) (Nat.ltb 0 (length (children node1))). *)
-(*   Eval compute in andb (is_debugging_tree node1) (Nat.ltb 0 (length (children node1))). *)
-(*   Definition top_down_strategy (n : Node) : (bool * Node) := *)
-(*     match correctness n with *)
-(*       no => match children n with *)
-(*              nil => (false, mkNode idk nil) *)
-(*            | _ => (true, hd (mkNode idk nil) (children n)) *)
-(*            end *)
-(*     | _ => (false, mkNode idk nil) *)
-(*     end. *)
-(*   (* Extraction top_down_strategy. *) *)
-(*   Eval compute in top_down_strategy node5. *)
-(*   Require Import Coq.Lists.List Coq.Bool.Bool. *)
-
-(*   Import Coq.Lists.List.ListNotations. *)
-
-(*   Scheme Equality for list. *)
-(*   Eval compute in Nat.ltb 1 2. *)
-(*   (* Eval compute in list_beq (Nat.leb) (1::nil) (1::nil). *) *)
-(*   (* Eval compute in list_beq (Nat.leb) (1::2::nil) (nil). *) *)
-(*   (* Fixpoint get_largest_nat_in_list_rec (largest : list nat) (l : list nat) : (list nat) := *) *)
-(*   (*   match l with *) *)
-(*   (*     nil => largest *) *)
-(*   (*   | head::tail => if (list_beq (nat) (Nat.leb) largest nil || (Nat.leb (hd 0 largest) head)) then get_largest_nat_in_list_rec (head::nil) tail else get_largest_nat_in_list_rec largest tail *) *)
-(*   (*   end. *) *)
-(*   (* Definition get_largest_nat_in_list (l : list nat) : (list nat) := *) *)
-(*   (*   get_largest_nat_in_list_rec [] l. *) *)
-(*   (* Eval compute in get_largest_nat_in_list_rec nil (0::1::7::8::9::3::4::5::nil). *) *)
-(*   (* Eval compute in get_largest_nat_in_list_rec nil (nil). *) *)
-(*   (* Eval compute in get_largest_nat_in_list (0::1::7::8::9::3::4::5::nil). *) *)
-(*   (* Eval compute in get_largest_nat_in_list (nil). *) *)
-(*   Check andb true. *)
-(*   Check weight . *)
-(*   (* Conseguir un typo Node -> bool *) *)
-(*   (* Eval compute in filter (weight Nat.eqb 2 ) (node1::nil). *) *)
-(*   Definition my_node_list : list Node := node1::node2::node3::node4::node5::nil. *)
-(*   (* Eval compute in filter (Nat.eqb weight list_max (map (fun n => weight n))) my_node_list. *) *)
-
-(*   Eval compute in list_max (nil). *)
-(*   (* Goal 0 * 0 = 2 -> False. *) *)
-(*   (* Proof. easy. *) *)
-(*   (* Qed. *) *)
-
-(*   Definition evaluate_node (n : Node) : Correctness := *)
-(*     no. *)
-(*   (* Lemma largest_of_list_is_correct: forall l: list nat, l <> nil -> get_largest_nat_in_list l <> nil. *) *)
-(*   (* Proof. intros l H. induction l. intuition. induction a. intuition. exact: (False_ind (0::l = [])). *) *)
-(*   (* Qed. *) *)
-(*   (* Definition get_heaviest_node (l : list Node, n : nat) : (bool * Node) := *) *)
-(*   (*   match l with *) *)
-(*   (*     nil => (false, mkNode idk nil) *) *)
-(*   (*     | *) *)
-(*   (* Definition heaviest_first_strategy (n : {n : Node | eq_true (andb (is_debugging_tree n) (Nat.ltb 0 (length (children n))))}) : Node := *) *)
-(*   (*   (hd (mkNode idk nil) (children (proj1_sig n))). *) *)
-(*   (* Eval compute in top_down_strategy node5. *) *)
-(*   (* Scheme Equality for Node. *) *)
-(*   (* Eval compute in Node_beq (mkNode no nil) (mkNode no nil). *) *)
-(*   Definition get_debugging_tree_from_tree (n : Node) : Node := *)
-(*     mkNode no (children n). *)
-
-(*   Fixpoint generic_debugging_algorithm (n : Node) : Node := *)
-(*     match children (get_debugging_tree_from_tree n) with *)
-(*       nil => n *)
-(*     | head::tail => generic_debugging_algorithm head *)
-(*     end. *)
-(*   (* Fixpoint choose A (l : list A) : distr A := *) *)
-(*   (*   match l with *) *)
-(*   (*     | nil => distr_null A *) *)
-(*   (*     | cons hd tl => Mchoice ([1/](length l)) (Munit hd) (choose tl) *) *)
-(*   (*   end. *) *)
-(*   (* Check is_true. *) *)
-(*   (* Lemma example2: forall a b: Prop, a/\b ->b/\a. *) *)
-(*   (*   Proof. intros a b H.  *) *)
-(*   (* Lemma generic_debugging_algorithm_is_correct : forall n : Node, children (generic_debugging_algorithm n) = nil. *) *)
-(*   (* Proof. intros. induction n. induction children0. *) *)
-(*   (*        + simpl. reflexivity. *) *)
-(*   (*        + simpl. *) *)
-(*   (* Definition remove_idk_node (l : list Node) (p : nat) : list Node := *) *)
-(*   (*   match l with *) *)
-(*   (*     nil => nil *) *)
-(*   (*     | _ => *) *)
-(*   (*   end. *) *)
-(*   (* (* Lemma choose_uniform : forall A (d : A) (l : list A) f, *) *) *)
-(*   (* (*   mu (choose l) f == sigma (fun i => ([1/](length l)) * f (nth i l d)) (length l). *) *) *)
-
-(*   (* (* Lemma In_nth : forall A (x:A) l, In x l -> exists i, (i < length l)%nat /\ nth i l x = x. *) *) *)
-
-(*   (* (* Lemma choose_le_Nnth : *) *) *)
-(*   (* (*   forall A (l:list A) x f alpha, *) *) *)
-(*   (* (*     In x l -> *) *) *)
-(*   (* (*     alpha <= f x -> *) *) *)
-(*   (* (*     [1/](length l) * alpha <= mu (choose l) f. *) *) *)
-
-(*   (* Section Gamble. *) *)
-
-(*   (* Fixpoint pow2 (n:nat) : nat := *) *)
-(*   (*    match n with O => 1%nat | S p => (2 * (pow2 p))%nat end. *) *)
-
-(*   (* Fixpoint play (n:nat) (b:nat) : distr nat := *) *)
-(*   (*     match n with *) *)
-(*   (*       O => Munit O *) *)
-(*   (*     | S p => Mif Flip (Munit ((pow2 n) * b)%nat) (play p (2*b)) *) *)
-(*   (*     end. *) *)
-
-(*   (* Lemma pow2not0 : forall n, pow2 n <> O. *) *)
-(*   (* induction n; simpl; omega. *) *)
-(*   (* Save. *) *)
-(*   (* Hint Resolve pow2not0. *) *)
-
-
-(*   (* Lemma proba_loose : forall n b, ~ b=O -> mu (play n b) (carac_eq O)== [1/2]^n. *) *)
-(*   (* induction n; intros. *) *)
-(*   (* simpl; auto. *) *)
-(*   (* simpl. *) *)
-(*   (* replace (pow2 n + (pow2 n + 0))%nat with (pow2 (S n)) by trivial. *) *)
-(*   (* rewrite (cover_eq_zero _ (is_eq O)). *) *)
-(*   (* repeat Usimpl. *) *)
-(*   (* apply IHn. *) *)
-(*   (* omega. *) *)
-(*   (* apply not_eq_sym. *) *)
-(*   (* apply NPeano.Nat.neq_mul_0; auto. *) *)
-(*   (* Save. *) *)
-
-(*   (* Lemma proba_win : forall n b, ~ b=O -> mu (play n b) (carac_eq ((pow2 n) * b)%nat)== [1-]([1/2]^n). *) *)
-(*   (* induction n; intros. *) *)
-(*   (* simpl; repeat Usimpl. *) *)
-(*   (* rewrite (cover_eq_zero _ (is_eq (b + 0))); intuition. *) *)
-(*   (* simpl. *) *)
-(*   (* rewrite (cover_eq_one _ (is_eq (pow2 (S n) * b)%nat)); trivial. *) *)
-(*   (* repeat Usimpl. *) *)
-(*   (* replace ((pow2 n + (pow2 n + 0)) * b)%nat with (pow2 n * (2*b))%nat. *) *)
-(*   (* rewrite IHn. *) *)
-(*   (* rewrite <- Uinv_half; repeat Usimpl; auto. *) *)
-(*   (* omega. *) *)
-(*   (* ring. *) *)
-(*   (* Save. *) *)
-
-(*   (* End Gamble. *) *)
-(*   Locate distr. *)
-(*   Fixpoint lrange n := *)
-(*     match n with *)
-(*     | O => cons O nil *)
-(*     | S m => cons (S m) (lrange m) *)
-(*     end. *)
-(*   Fixpoint choose A (l : list A) : distr A := *)
-(*     match l with *)
-(*     | nil => distr_null A *)
-(*     | cons hd tl => Mchoice ([1/]1+(length l)) (Munit hd) (choose tl) *)
-(*     end. *)
-
-(*   Check choose (lrange (S 0)). *)
-(*   Check choose (yes::no::nil). *)
-(*   Search distr. *)
-
-(* End MyM. *)
+Proof.
+  intros n.
+  induction n.
+  induction children0.
+  + simpl generic_debugging_algorithm. Tactics.program_simpl. simpl. intuition. auto. eauto.
